src/Reflection/CommonSubexpressionElimination.v
@@ -1,0 +1,198 @@
+(** * Common Subexpression Elimination for PHOAS Syntax *)
+Require Import Coq.Lists.List.
+Require Import Crypto.Reflection.Syntax.
+Require Import Crypto.Util.Tactics Crypto.Util.Bool.
+
+Local Open Scope list_scope.
+
+Inductive symbolic_expr {base_type_code SConstT op_code} : Type :=
+| SConst (v : SConstT)
+| SVar   (v : base_type_code) (n : nat)
+| SOp    (op : op_code) (args : symbolic_expr)
+| SPair  (x y : symbolic_expr)
+| SInvalid.
+Scheme Equality for symbolic_expr.
+
+Arguments symbolic_expr : clear implicits.
+
+Ltac inversion_symbolic_expr_step :=
+  match goal with
+  | [ H : SConst _ = SConst _ |- _ ] => inversion H; clear H
+  | [ H : SVar _ _ = SVar _ _ |- _ ] => inversion H; clear H
+  | [ H : SOp _ _ = SOp _ _ |- _ ] => inversion H; clear H
+  | [ H : SPair _ _ = SPair _ _ |- _ ] => inversion H; clear H
+  end.
+Ltac inversion_symbolic_expr := repeat inversion_symbolic_expr_step.
+
+Local Open Scope ctype_scope.
+Section symbolic.
+  (** Holds decidably-equal versions of raw expressions, for lookup. *)
+  Context (base_type_code : Type)
+          (SConstT : Type)
+          (op_code : Type)
+          (base_type_code_beq : base_type_code -> base_type_code -> bool)
+          (SConstT_beq : SConstT -> SConstT -> bool)
+          (op_code_beq : op_code -> op_code -> bool)
+          (base_type_code_bl : forall x y, base_type_code_beq x y = true -> x = y)
+          (base_type_code_lb : forall x y, x = y -> base_type_code_beq x y = true)
+          (SConstT_bl : forall x y, SConstT_beq x y = true -> x = y)
+          (SConstT_lb : forall x y, x = y -> SConstT_beq x y = true)
+          (op_code_bl : forall x y, op_code_beq x y = true -> x = y)
+          (op_code_lb : forall x y, x = y -> op_code_beq x y = true)
+          (interp_base_type : base_type_code -> Type)
+          (op : flat_type base_type_code -> flat_type base_type_code -> Type)
+          (symbolize_const : forall t, interp_base_type t -> SConstT)
+          (symbolize_op : forall s d, op s d -> op_code).
+
+  Local Notation symbolic_expr := (symbolic_expr base_type_code SConstT op_code).
+  Local Notation symbolic_expr_beq := (@symbolic_expr_beq base_type_code SConstT op_code base_type_code_beq SConstT_beq op_code_beq).
+  Local Notation symbolic_expr_lb := (@internal_symbolic_expr_dec_lb base_type_code SConstT op_code base_type_code_beq SConstT_beq op_code_beq base_type_code_lb SConstT_lb op_code_lb).
+  Local Notation symbolic_expr_bl := (@internal_symbolic_expr_dec_bl base_type_code SConstT op_code base_type_code_beq SConstT_beq op_code_beq base_type_code_bl SConstT_bl op_code_bl).
+
+  Local Notation flat_type := (flat_type base_type_code).
+  Local Notation type := (type base_type_code).
+  Let Tbase := @Tbase base_type_code.
+  Local Coercion Tbase : base_type_code >-> flat_type.
+  Local Notation interp_type := (interp_type interp_base_type).
+  Local Notation interp_flat_type := (interp_flat_type_gen interp_base_type).
+  Local Notation exprf := (@exprf base_type_code interp_base_type op).
+  Local Notation expr := (@expr base_type_code interp_base_type op).
+  Local Notation Expr := (@Expr base_type_code interp_base_type op).
+
+
+  Section with_var.
+    Context {var : base_type_code -> Type}.
+
+    Local Notation svar t := (var t * symbolic_expr)%type.
+    Local Notation fsvar := (fun t => svar t).
+    Local Notation mapping := (forall t : base_type_code, list (svar t))%type.
+
+    Context (prefix : list (sigT (fun t : flat_type => @exprf fsvar t))).
+
+    Definition empty_mapping : mapping := fun _ => nil.
+    Definition type_lookup t (xs : mapping) : list (svar t) := xs t.
+    Definition mapping_update_type t (xs : mapping) (upd : list (svar t) -> list (svar t))
+      : mapping
+      := fun t' => (if base_type_code_beq t t' as b return base_type_code_beq t t' = b -> _
+                    then fun H => match base_type_code_bl _ _ H in (_ = t') return list (svar t') with
+                                  | eq_refl => upd (type_lookup t xs)
+                                  end
+                    else fun _ => type_lookup t' xs)
+                     eq_refl.
+
+    Fixpoint lookup' {t} (sv : symbolic_expr) (xs : list (svar t)) {struct xs} : option (var t) :=
+      match xs with
+      | nil => None
+      | (x, sv') :: xs' =>
+        if symbolic_expr_beq sv' sv
+        then Some x
+        else lookup' sv xs'
+      end.
+    Definition lookup t (sv : symbolic_expr) (xs : mapping) : option (var t) :=
+      lookup' sv (type_lookup t xs).
+    Definition symbolicify_var {t : base_type_code} (v : var t) (xs : mapping) : symbolic_expr :=
+      SVar t (length (type_lookup t xs)).
+    Definition add_mapping {t} (v : var t) (sv : symbolic_expr) (xs : mapping) : mapping :=
+      mapping_update_type t xs (fun ls => (v, sv) :: ls).
+
+    Definition symbolize_smart_const {t} : interp_flat_type t -> symbolic_expr
+      := smart_interp_flat_map base_type_code (g:=fun _ => symbolic_expr) (fun t v => SConst (symbolize_const t v)) (fun A B => SPair).
+
+    Fixpoint symbolize_exprf
+             {t} (v : @exprf fsvar t) {struct v}
+      : option symbolic_expr
+      := match v with
+         | Const t x => Some (symbolize_smart_const x)
+         | Var _ x => Some (snd x)
+         | Op _ _ op args => option_map
+                               (fun sargs => SOp (symbolize_op _ _ op) sargs)
+                               (@symbolize_exprf _ args)
+         | Let _ ex _ eC => None
+         | Pair _ ex _ ey => match @symbolize_exprf _ ex, @symbolize_exprf _ ey with
+                             | Some sx, Some sy => Some (SPair sx sy)
+                             | _, _ => None
+                             end
+         end.
+
+    Fixpoint smart_lookup_gen f (proj : forall t, svar t -> f t)
+             (t : flat_type) (sv : symbolic_expr) (xs : mapping) {struct t}
+      : option (interp_flat_type_gen f t)
+      := match t return option (interp_flat_type_gen f t) with
+         | Syntax.Tbase t => option_map (fun v => proj t (v, sv)) (lookup t sv xs)
+         | Prod A B => match @smart_lookup_gen f proj A sv xs, @smart_lookup_gen f proj B sv xs with
+                       | Some a, Some b => Some (a, b)
+                       | _, _ => None
+                       end
+         end.
+    Definition smart_lookup (t : flat_type) (sv : symbolic_expr) (xs : mapping) : option (interp_flat_type_gen fsvar t)
+      := @smart_lookup_gen fsvar (fun _ x => x) t sv xs.
+    Definition smart_lookupo (t : flat_type) (sv : option symbolic_expr) (xs : mapping) : option (interp_flat_type_gen fsvar t)
+      := match sv with
+         | Some sv => smart_lookup t sv xs
+         | None => None
+         end.
+    Definition symbolicify_smart_var {t : flat_type} (xs : mapping) (replacement : option symbolic_expr)
+      : interp_flat_type_gen var t -> interp_flat_type_gen fsvar t
+      := smart_interp_flat_map
+           (g:=interp_flat_type_gen fsvar)
+           base_type_code (fun t v => (v,
+                                       match replacement with
+                                       | Some sv => sv
+                                       | None => symbolicify_var v xs
+                                       end))
+           (fun A B => @pair _ _).
+    Fixpoint smart_add_mapping {t : flat_type} (xs : mapping) : interp_flat_type_gen fsvar t -> mapping
+      := match t return interp_flat_type_gen fsvar t -> mapping with
+         | Syntax.Tbase t => fun v => add_mapping (fst v) (snd v) xs
+         | Prod A B
+           => fun v => let xs := @smart_add_mapping B xs (snd v) in
+                       let xs := @smart_add_mapping A xs (fst v) in
+                       xs
+         end.
+
+    Definition csef_step
+               (csef : forall {t} (v : @exprf fsvar t) (xs : mapping), @exprf var t)
+               {t} (v : @exprf fsvar t) (xs : mapping)
+      : @exprf var t
+      := match v in @Syntax.exprf _ _ _ _ t return exprf t with
+         | Let tx ex _ eC => let sx := symbolize_exprf ex in
+                             let ex' := @csef _ ex xs in
+                             let sv := smart_lookupo tx sx xs in
+                             match sv with
+                             | Some v => @csef _ (eC v) xs
+                             | None
+                               => Let ex' (fun x => let x' := symbolicify_smart_var xs sx x in
+                                                    @csef _ (eC x') (smart_add_mapping xs x'))
+                             end
+         | Const _ x => Const x
+         | Var _ x => Var (fst x)
+         | Op _ _ op args => Op op (@csef _ args xs)
+         | Pair _ ex _ ey => Pair (@csef _ ex xs) (@csef _ ey xs)
+         end.
+
+    Fixpoint csef {t} (v : @exprf fsvar t) (xs : mapping)
+      := @csef_step (@csef) t v xs.
+
+    Fixpoint prepend_prefix {t} (e : @exprf fsvar t) (ls : list (sigT (fun t : flat_type => @exprf fsvar t)))
+      : @exprf fsvar t
+      := match ls with
+         | nil => e
+         | x :: xs => Let (projT2 x) (fun _ => @prepend_prefix _ e xs)
+         end.
+
+    Fixpoint cse {t} (v : @expr fsvar t) (xs : mapping) {struct v} : @expr var t
+      := match v in @Syntax.expr _ _ _ _ t return expr t with
+         | Return _ x => Return (csef (prepend_prefix x prefix) xs)
+         | Abs _ _ f => Abs (fun x => let x' := symbolicify_var x xs in
+                                      @cse _ (f (x, x')) (add_mapping x x' xs))
+         end.
+  End with_var.
+
+  Definition CSE {t} (e : Expr t) (prefix : forall var, list (sigT (fun t : flat_type => @exprf var t)))
+    : Expr t
+    := fun var => cse (prefix _) (e _) empty_mapping.
+End symbolic.
+
+Global Arguments csef {_} SConstT op_code base_type_code_beq SConstT_beq op_code_beq base_type_code_bl {_ _} symbolize_const symbolize_op {var t} _ _.
+Global Arguments cse {_} SConstT op_code base_type_code_beq SConstT_beq op_code_beq base_type_code_bl {_ _} symbolize_const symbolize_op {var} prefix {t} _ _.
+Global Arguments CSE {_} SConstT op_code base_type_code_beq SConstT_beq op_code_beq base_type_code_bl {_ _} symbolize_const symbolize_op {t} e prefix var.
